another stable place

src/SDK/Serialize/Header.dfy
@@ -5,21 +5,103 @@ include "../../Generated/AwsCryptographicMaterialProviders.dfy"
 include "../../AwsCryptographicMaterialProviders/Client.dfy"
 include "../../StandardLibrary/StandardLibrary.dfy"
 include "../../Util/UTF8.dfy"
-include "./SerializableTypes.dfy"
+include "SerializableTypes.dfy"
 include "SerializeFunctions.dfy"
 include "EncryptionContext.dfy"
+
+include "V1HeaderBody.dfy"
+include "V2HeaderBody.dfy"
+include "HeaderTypes.dfy"
+include "HeaderAuth.dfy"
+include "SharedHeaderFunctions.dfy"
+
 
 module Header {
   import Aws.Crypto
   import Seq
   import MaterialProviders.Client
   import EncryptionContext2
+
+  import V1HeaderBody
+  import V2HeaderBody
+  import HeaderTypes
+  import HeaderAuth
+  import SharedHeaderFunctions
+
   import opened SerializableTypes
   import opened StandardLibrary.UInt
   import opened Wrappers
   import opened UTF8
   import opened SerializeFunctions
 
+datatype HeaderInfo = HeaderInfo(
+    nameonly body: HeaderTypes.HeaderBody,
+    nameonly rawHeader: seq<uint8>,
+    nameonly suite: Client.AlgorithmSuites.AlgorithmSuite,
+    nameonly headerAuth: HeaderTypes.HeaderAuth
+  )
 
+  type Header = h: HeaderInfo
+  |
+    && GetESDKAlgorithmSuiteId(h.suite.id) == h.body.esdkSuiteId
+    && h.body.contentType.NonFramed? <==> 0 == h.body.frameLength
+    && h.body.contentType.Framed? <==> 0 < h.body.frameLength
+    && (h.headerAuth.AESMac?
+    ==>
+      && |h.headerAuth.headerIv| == h.suite.encrypt.ivLength as nat
+      && |h.headerAuth.headerAuthTag| == h.suite.encrypt.tagLength as nat)
+    && (h.suite.commitment.HKDF?
+      ==>
+        && h.body.V2HeaderBody?
+        && |h.body.suiteData| == h.suite.commitment.outputKeyLength as nat)
+    && (!h.suite.commitment.HKDF?
+      ==>
+        && h.body.V1HeaderBody?)
+    && CorrectlyReadHeaderBody(h.body, ReadableBytes(h.rawHeader, 0))
+  witness *
+
+  function method ReadHeaderBody(
+     bytes: ReadableBytes
+  )
+    :(res: ReadCorrect<HeaderTypes.HeaderBody>)
+    ensures res.Success? ==> CorrectlyReadHeaderBody(res.value.thing, bytes)
+  {
+
+    var version :- SharedHeaderFunctions.ReadMessageFormatVersion(bytes);
+
+    match version.thing
+    case V1 => 
+      var b :- V1HeaderBody.ReadV1HeaderBody(bytes);
+      var body: HeaderTypes.HeaderBody := b.thing;
+      Success(Data(body, b.tail))
+    case V2 => 
+      var b :- V2HeaderBody.ReadV2HeaderBody(bytes);
+      var body: HeaderTypes.HeaderBody := b.thing;
+      Success(Data(body, b.tail))
+  }
+
+  predicate CorrectlyReadHeaderBody(
+    body: HeaderTypes.HeaderBody,
+    bytes: ReadableBytes
+  )
+  {
+    match body
+    case V1HeaderBody(_,_,_,_,_,_,_,_) =>
+      V1HeaderBody.CorrectlyReadV1HeaderBody(bytes, Success(Data(body, bytes)))
+    case V2HeaderBody(_,_,_,_,_,_,_) =>
+      V2HeaderBody.CorrectlyReadV2HeaderBody(bytes, Success(Data(body, bytes)))
+  }
+
+  function method WriteHeaderBody(
+    body: HeaderTypes.HeaderBody
+  )
+    :(ret: seq<uint8>)
+  {
+    match body
+    case V1HeaderBody(_,_,_,_,_,_,_,_) =>
+      V1HeaderBody.WriteV1HeaderBody(body)
+    case V2HeaderBody(_,_,_,_,_,_,_) =>
+      V2HeaderBody.WriteV2HeaderBody(body)
+  }
 
 }
